Main.lean
@@ -1,0 +1,150 @@
+import cvc5
+
+
+
+namespace cvc5.Test
+
+
+
+namespace RaceCondition
+
+def context (blah : String) (code : ReaderT σ (EST Error ω) α) : ReaderT σ (EST Error ω) α :=
+  fun state world =>
+    match code state world with
+    | .ok res state => .ok res state
+    | .error Error.missingValue state => .error (Error.error s!"{blah}\nmissing value") state
+    | .error (Error.error err) state
+    | .error (Error.recoverable err) state
+    | .error (Error.option err) state
+    | .error (Error.unsupported err) state => .error (Error.error s!"{blah}\n{err}") state
+
+
+def Mem (ω : Type) (α : Type) [BEq α] [Hashable α] := ST.Ref ω (Std.HashSet α)
+
+namespace Mem variable [BEq α] [Hashable α]
+
+protected abbrev IO := Mem IO.RealWorld
+
+def empty : BaseIO (Mem.IO α) := ST.mkRef <| Std.HashSet.emptyWithCapacity 1000
+
+def insert (i : α) (mem : Mem ω α) : ST ω Unit := do
+  mem.modifyGet fun set => ((), set.insert i)
+
+def checkVals (f : α → ExceptT String IO Unit) (mem : Mem.IO α) : ExceptT String IO Unit := do
+  let map ← mem.get
+  for val in map do f val
+
+end Mem
+
+def mkNeInt (term : Term) (val : Int) : Term.Env ω Term := do
+  let sortKind := term.getSort.getKind
+  if sortKind != .INTEGER_SORT then
+    throw <| Error.error s!"term `{term}` has type `{term.getSort}`, expected `Int`"
+  let rhs : Term ← Term.Manager.mkInteger! val |> context s!"mkInteger! {val}"
+  let eqTerm ← Term.Manager.mkTerm .EQUAL #[term, rhs] |> context s!"mkTerm .EQUAL .."
+  Term.Manager.mkTerm .NOT #[eqTerm] |> context s!"mkTerm .NOT .."
+
+def randInt (normMax : Nat := 1000) : BaseIO Int := do
+  let n ← IO.rand 0 normMax
+  let neg ← (· == 1) <$> IO.rand 0 1
+  return if neg then - n else n
+
+def genTerm (lhs : Term) (valMem : Mem.IO Int) (normMax : Nat := 1000) : Term.Env.IO Term := do
+  let i ← randInt normMax
+  valMem.insert i
+  mkNeInt lhs i
+
+def genTerms (n : Nat) (lhs : Term)
+  (valMem : Mem.IO Int) (termMem : Mem.IO Term) (normMax : Nat := 1000)
+: Term.Env.IO Unit := do
+  for _ in [0:n] do
+    let term ← genTerm lhs valMem normMax |> context "during term gen"
+    termMem.insert term
+
+
+
+def runTest (taskCount : Nat) (genCount : Nat) (normMax : Nat := 1000) : IO Unit := do
+  -- stores `Int` values
+  let valMem ← Mem.empty
+  -- stores `Term` values
+  let termMem ← Mem.empty
+
+  let manager ← Term.mkManager
+
+  let x ← manager.run! do
+    let intSort ← Term.Manager.getIntegerSort
+    Term.Manager.mkConst intSort "x"
+  println! "created `{x} : {x.getSort}`"
+
+  println! "spawning {taskCount} tasks to `{x} ≠ i` terms for {genCount} random values of `i : Int`"
+  let mut termTasks := Array.emptyWithCapacity taskCount
+  for n in [0:taskCount] do
+    let task ← IO.asTask do
+      manager.run! (genTerms genCount x valMem termMem normMax)
+      println! "  thread #{n.succ} is done"
+    termTasks := termTasks.push task
+  println! "waiting for tasks to finish"
+  for task in termTasks do
+    match task.get with
+    | .ok () => pure ()
+    | .error e =>
+      println! "an error occurred"
+      println! "  {e}"
+      return ()
+
+  let valCount := (← valMem.get).size
+  let termCount := (← termMem.get).size
+  println! "created {termCount} different term(s) --- {valCount} different value(s)"
+
+  let solver ← manager.mkSolver
+
+  solver.run! (Cvc.setOption "produce-models" "true")
+
+  println! "asserting all terms"
+  -- let mut assertTasks := Array.emptyWithCapacity taskCount
+  let mut cnt := 0
+  for term in ← termMem.get do
+    let n := cnt
+    cnt := cnt + 1
+    -- let task ← IO.asTask do
+    solver.run! (Cvc.assertFormula term)
+    println! "  thread #{n.succ} is done"
+    -- assertTasks := assertTasks.push task
+  -- wait for tasks to finish
+  -- for task in assertTasks do
+  --   match task.get with
+  --   | .ok () => pure ()
+  --   | .error e => throw e
+  println! "all assertion tasks done"
+
+  -- done, get a value for `x`
+  let value ← solver.run! do
+    let result ← Cvc.checkSat
+    if ¬ result.isSat then
+      throw <| Error.error "expected sat result 🙀"
+    let value ← Cvc.getValue x
+    if let some value := value.getIntegerValue?
+    then pure value
+    else throw <| Error.error s!"unexpected value for `x`: `{value}`"
+
+  println! "got a value for `x`: `{value}`"
+  -- if everything went fine, `value` should be different from all `Int`s in `valMem`
+  let ok? ← valMem.checkVals fun i => do
+    if i = value then .error s!"`valMem` indicates value `{value}` is impossible for `x`"
+    else
+      println! "- confirmed ≠ {i}"
+      pure ()
+  if let .error e := ok? then
+    println! "❌ something went wrong:"
+    println! "{e}"
+  else
+    println! "✅ all good"
+
+  println! "done"
+
+
+
+-- #eval runTest 10 300
+
+def _root_.main : IO Unit :=
+  cvc5.Test.RaceCondition.runTest 10 10 100_000
