lakefile.lean
@@ -127,3 +127,6 @@ lean_lib cvc5 where
 @[test_driver]
 lean_lib cvc5Test where
   globs := #[Glob.submodules `cvc5Test]
+
+lean_exe testing where
+  root := `Main
